lang.v
@@ -303,9 +303,6 @@ Module F_mu_ref_conc.
            fill_item_val, fill_item_no_val_inj, head_ctx_step_val.
   Qed.
 
-  Canonical Structure stateC := leibnizC state.
-  Canonical Structure valC := leibnizC val.
-  Canonical Structure exprC := leibnizC expr.
 End F_mu_ref_conc.
 
 Canonical Structure F_mu_ref_conc_ectxi_lang :=
