rules.v
@@ -60,7 +60,7 @@ Section lang_rules.
     iIntros (<- Φ) "_ HΦ". iApply wp_lift_atomic_head_step_no_fork; auto.
     iIntros (σ1 ???) "Hσ !>"; iSplit; first by auto.
     iNext; iIntros (v2 σ2 efs Hstep); inv_head_step.
-    iMod (@gen_heap_alloc with "Hσ") as "[Hσ Hl]"; first done.
+    iMod (@gen_heap_alloc with "Hσ") as "[Hσ [Hl ?]]"; first done.
     iModIntro; iSplit=> //. iFrame. by iApply "HΦ".
   Qed.
 
